AllNoNotations.v
@@ -1,2 +1,2 @@
-Require Export bbv.Word bbv.HexNotationWord Rtl Compile Lib.Fold Lib.EclecticLib Utila RecordUpdate.RecordSet.
+Require Export Lib.Word Lib.HexNotationWord Rtl Compile Lib.Fold Lib.EclecticLib Utila RecordUpdate.RecordSet.
 Require Export Syntax Properties PProperties PPlusProperties Extraction Tactics.
