Lib/HexNotationWord.v
@@ -1,0 +1,35 @@
+Require Export Lib.Word.
+Require Export Lib.HexNotation.
+Require Export Lib.Word.
+Export Word.Notations.
+Open Scope word_scope.
+Require Import Coq.ZArith.BinIntDef Coq.ZArith.BinInt Coq.ZArith.Zdiv.
+
+
+Notation "'Ox' a" := (NToWord _ (hex a)) (at level 50).
+
+Notation "sz ''h' a" := (NToWord sz (hex a)) (at level 50).
+
+Goal 8'h"a" = zToWord 8 (wordVal _ (NToWord 4 10)).
+Proof.
+  reflexivity.
+Qed.
+
+Goal Ox"41" = zToWord 7 65.
+Proof.
+  reflexivity.
+Qed.
+
+Notation "sz ''b' a" := (zToWord sz (Z.of_nat (bin a))) (at level 50).
+
+Notation "''b' a" := (zToWord _ (Z.of_nat (bin a))) (at level 50).
+
+Goal 'b"00001010" = zToWord 8 (wordVal _ (NToWord 4 10)).
+Proof.
+  reflexivity.
+Qed.
+
+Goal 'b"1000001" = zToWord 7 65.
+Proof.
+  reflexivity.
+Qed.
